Kami/Ex/ProcDecInl.v
@@ -25,7 +25,7 @@ Section Inlined.
             (alignPc: AlignPcT addrSize iaddrSize)
             (alignAddr: AlignAddrT addrSize).
 
-  Variable (init: ProcInit addrSize iaddrSize dataBytes rfIdx).
+  Variable (init: ProcInit addrSize dataBytes rfIdx).
 
   Definition pdec := pdecf fifoSize getOptype getLdDst getLdAddr getLdSrc calcLdAddr
                            getStAddr getStSrc calcStAddr getStVSrc
