Kami/Ex/ProcDecInv.v
@@ -33,7 +33,7 @@ Section Invariants.
   Definition RqFromProc := MemTypes.RqFromProc dataBytes (Bit addrSize).
   Definition RsToProc := MemTypes.RsToProc dataBytes.
 
-  Variable (init: ProcInit addrSize iaddrSize dataBytes rfIdx).
+  Variable (init: ProcInit addrSize dataBytes rfIdx).
 
   Definition pdecInl := pdecInl fifoSize getOptype getLdDst getLdAddr getLdSrc calcLdAddr
                                 getStAddr getStSrc calcStAddr getStVSrc
