Kami/Ex/ProcFDInl.v
@@ -58,14 +58,13 @@ Section Inlined.
     (f2dEpoch: forall ty, fullType ty (SyntaxKind f2dElt) ->
                           Expr ty (SyntaxKind Bool)).
 
-  Variables (pcInit : ConstT (Bit addrSize))
-            (pgmInit : ConstT (Vector (Data dataBytes) iaddrSize)).
+  Variables (pcInit : ConstT (Bit addrSize)).
 
   Definition fetchDecode := fetchDecode getOptype getLdDst getLdAddr getLdSrc calcLdAddr
                                         getStAddr getStSrc calcStAddr getStVSrc
                                         getSrc1 getSrc2 getDst alignPc predictNextPc
                                         d2ePack f2dPack f2dRawInst f2dCurPc f2dNextPc f2dEpoch
-                                        pcInit pgmInit.
+                                        pcInit.
   Hint Unfold fetchDecode: ModuleDefs. (* for kinline_compute *)
 
   Definition fetchDecodeInl: sigT (fun m: Modules => fetchDecode <<== m).
@@ -75,8 +74,7 @@ Section Inlined.
                                         getStAddr getStSrc calcStAddr getStVSrc
                                         getSrc1 getSrc2 getDst alignPc predictNextPc d2ePack
                                         f2dPack f2dRawInst f2dCurPc f2dNextPc f2dEpoch
-                                        pcInit pgmInit
-                                        type typeUT)
+                                        pcInit type typeUT)
                   (Reflection.noDupStr_NoDup (Struct.namesOf (getDefsBodies fetchDecode)) eq_refl))
       as Him.
     unfold MethsT in Him; rewrite <-SemFacts.idElementwiseId in Him.
